src/lang/Progress.v
@@ -73,8 +73,8 @@ Lemma progress_promise_step
       (WF1: Local.wf lc1 mem1)
       (MEM1: Memory.closed mem1)
       (SC1: Memory.closed_timemap sc1 mem1)
-      (WF_REL: View.wf releasedm)
-      (CLOSED_REL: Memory.closed_view releasedm mem1):
+      (WF_REL: View.opt_wf releasedm)
+      (CLOSED_REL: Memory.closed_opt_view releasedm mem1):
   exists promises2 mem2,
     Local.promise_step lc1 mem1 loc (Memory.max_ts loc mem1) to val
                        (TView.write_released (Local.tview lc1) sc1 loc to releasedm ord)
@@ -96,12 +96,13 @@ Proof.
       (try by left; eapply TimeFacts.le_lt_lt; [|eauto];
        eapply closed_timemap_max_ts; apply WF1).
     left. eapply TimeFacts.le_lt_lt; [|eauto].
-    eapply closed_timemap_max_ts. apply CLOSED_REL.
-  - unfold TView.write_released.
+    eapply closed_timemap_max_ts. apply Memory.unwrap_closed_opt_view; viewtac.
+  - unfold TView.write_released. condtac; econs.
     viewtac;
       repeat condtac; viewtac;
         (try eapply Memory.add_closed_view; eauto);
         (try apply WF1).
+    + viewtac.
     + erewrite Memory.add_o; eauto. condtac; eauto. ss. des; congr.
     + econs; try apply Memory.closed_timemap_bot; viewtac.
     + erewrite Memory.add_o; eauto. condtac; eauto. ss. des; congr.
@@ -119,7 +120,7 @@ Proof.
   exploit (Memory.max_ts_spec loc); try apply MEM1; eauto. i. des.
   esplits; eauto. econs; eauto.
   econs; try by i; eapply Memory.max_ts_spec2; apply WF1.
-  i. eapply Memory.max_ts_spec2. eapply MEM1. eauto.
+  i. eapply Memory.max_ts_spec2. apply Memory.unwrap_closed_opt_view; viewtac. eapply MEM1. eauto.
 Qed.
 
 Lemma progress_write_step
@@ -129,8 +130,8 @@ Lemma progress_write_step
       (WF1: Local.wf lc1 mem1)
       (SC1: Memory.closed_timemap sc1 mem1)
       (MEM1: Memory.closed mem1)
-      (WF_REL: View.wf releasedm)
-      (CLOSED_REL: Memory.closed_view releasedm mem1)
+      (WF_REL: View.opt_wf releasedm)
+      (CLOSED_REL: Memory.closed_opt_view releasedm mem1)
       (PROMISES1: lc1.(Local.promises) = Memory.bot):
   exists released lc2 sc2 mem2,
     Local.write_step lc1 sc1 mem1 loc (Memory.max_ts loc mem1) to val releasedm released ord lc2 sc2 mem2 Memory.op_kind_add.
